Request generator

app/Execute.v
@@ -3,16 +3,16 @@ From HTTP Require Import
 From App Require Import
      Tester.
 
-Variant texp : Type -> Set :=
+Variant texp : Type -> Type :=
   Texp__Const   : N -> texp N
-| Texp__Order   : labelT -> texp N
-| Texp__Account : labelT -> nat -> texp N
-| Texp__Amount  : labelT -> nat -> N -> texp N.
+| Texp__Order   : labelT -> nat -> texp order_id
+| Texp__Account : labelT -> nat -> texp account_id
+| Texp__Amount  : labelT -> nat -> N -> texp amountT.
 
 Instance Serialize__texp : Serialize (texp N) :=
   fun tx => match tx with
          | Texp__Const    n   => Atom n
-         | Texp__Order    x   => [Atom "Order"; Atom x]
+         | Texp__Order    x n => [Atom "Order"  ; Atom x; Atom n]
          | Texp__Account  x n => [Atom "Account"; Atom x; Atom n]
          | Texp__Amount x n p => [Atom "Amount" ; Atom x; Atom n; Atom p]
          end%sexp.
@@ -32,7 +32,30 @@ Instance Serialize__request {exp_} `{Serialize (exp_ N)}
 
 Instance Serialize__symreq : Serialize (swap_request texp) := Serialize__request.
 
-Instance Shrink__request : Shrink (swap_request texp) := { shrink _ := [] }.
+Instance Shrink__texp : Shrink (texp N) := {
+  shrink x :=
+    match x with
+    | Texp__Const      n => Texp__Const   <$> shrink n
+    | Texp__Order    x n => Texp__Order x <$> shrink n ++
+                         Texp__Order   <$> shrink x <*> [n]
+    | Texp__Account  x n => Texp__Account x <$> shrink n ++
+                         Texp__Account   <$> shrink x <*> [n]
+    | Texp__Amount x n p => Texp__Amount x n <$> shrink p ++
+                         Texp__Amount x   <$> shrink n <*> [p] ++
+                         Texp__Amount     <$> shrink x <*> [n] <*> [p]
+    end }.
+
+Instance Shrink__request : Shrink (swap_request texp) :=
+  { shrink req :=
+      match req with
+      | Request__TakeOrder u o => Request__TakeOrder u <$> shrink o
+      | Request__MakeOrder u bt ba st sa =>
+        Request__MakeOrder u bt ba st <$> shrink sa ++
+        Request__MakeOrder u bt       <$> shrink ba <*> [st] <*> [sa]
+      | Request__Deposit   u t a => Request__Deposit  u t <$> shrink a
+      | Request__Withdraw  u t a => Request__Withdraw u t <$> shrink a
+      | _ => []
+      end }.
 
 Notation packetT := (packetT (swap_request id) (swap_response id)).
 Notation traceT  := (@traceT packetT).
@@ -41,3 +64,105 @@ Fixpoint fallback {A B} (f : A -> option B) (l : list A) : B -> B :=
   if l is a::l'
   then if f a is Some b then const b else fallback f l'
   else id.
+
+Definition instantiate_exp (tr : traceT) (nx : texp N) : N :=
+  match nx with
+  | Texp__Const n => n
+  | Texp__Order l k =>
+    fallback
+      (fun lp =>
+         let '(l0, Packet _ _ p) := lp in
+         if l0 = l? then
+           match p with
+           | inr (Response__Order (n, _)) => Some n
+           | inr (Response__ListOrders l) =>
+             fst <$> nth_error l (min k (pred (length l)))
+           | _ => None
+           end
+         else None) tr 0
+  | Texp__Account l k =>
+    fallback
+      (fun lp =>
+         let '(l0, Packet _ _ p) := lp in
+         if l0 = l? then
+           match p with
+           | inr (Response__Account (n, _)) => Some n
+           | inr (Response__ListAccount l)  =>
+             fst <$> nth_error l (min k (pred (length l)))
+           | _ => None
+           end
+         else None) tr 0
+  | Texp__Amount l k x =>
+    (fallback
+      (fun lp =>
+         let '(l0, Packet _ _ p) := lp in
+         if l0 = l? then
+           match p with
+           | inr (Response__Account (_, (_, _, a))) => Some a
+           | inr (Response__ListAccount l) =>
+             snd ∘ snd <$> nth_error l (min k (pred (length l)))
+           | _ => None
+           end
+         else None) tr 100) * x / 4
+  end.
+
+Definition instantiate_request (tr : traceT) (rx : swap_request texp)
+  : swap_request id :=
+  match rx with
+  | Request__ListOrders =>
+    Request__ListOrders
+  | Request__ListAccount uid =>
+    Request__ListAccount uid
+  | Request__TakeOrder   uid ox =>
+    Request__TakeOrder   uid          $ instantiate_exp tr ox
+  | Request__MakeOrder   uid bt ba st sax =>
+    Request__MakeOrder   uid bt ba st $ instantiate_exp tr sax
+  | Request__Deposit     uid t a =>
+    Request__Deposit     uid t a
+  | Request__Withdraw    uid t ax =>
+    Request__Withdraw    uid t        $ instantiate_exp tr ax
+  end.
+
+Definition randomN : N -> IO N := fmap n_of_int ∘ ORandom.int ∘ int_of_n.
+
+Definition gen_request (ss : swap_state exp) (tr : traceT)
+  : IO (swap_request texp) :=
+  let (accounts, orders) := ss in
+  let getOrder (lp : labelT * packetT) : IO (option (texp order_id)) :=
+      let '(l, Packet _ _ p) := lp in
+      match p with
+      | inr (Response__Order _) => ret $ Some (Texp__Order l O)
+      | inr (Response__ListOrders ((_::_) as os)) =>
+        Some ∘ Texp__Order l ∘ fst <$> io_choose' os
+      | _ => ret None
+      end in
+  let genOrder : IO order_id :=
+      let getOid (o : orderT exp) : option order_id :=
+          if fst o is Exp__Const n then Some n else None in
+      io_choose_ (ret 0) (map_if getOid orders) in
+  let getAmount (lp : labelT * packetT) : IO (option (texp amountT)) :=
+      let '(l, Packet _ _ p) := lp in
+      pc <- randomN 8;;
+      match p with
+      | inr (Response__Account _) => ret $ Some (Texp__Amount l O pc)
+      | inr (Response__ListAccount ((_::_) as la)) =>
+             Some <$> (Texp__Amount l <$> (fst <$> io_choose' la) <*> (ret pc))
+      | _ => ret None
+      end in
+  let genAmount : IO amountT :=
+      io_choose_ (ret 100) (map (snd ∘ snd) accounts) in
+  uid <- io_choose [0;1;2;3;4];;
+  lox <- map_if id <$> sequence (map getOrder tr);;
+  oid <- io_choose_ (Texp__Const <$> genOrder) lox;;
+  bt <- io_choose ["CNY";"USD";"JPY";"EUR";"ETH"];;
+  ba <- randomN 1000;;
+  st <- io_choose ["CNY";"USD";"JPY";"EUR";"ETH"];;
+  ams <- map_if id <$> sequence (map getAmount tr);;
+  ax <- io_choose_ (Texp__Const <$> genAmount) ams;;
+  io_choose
+    [Request__ListOrders;
+     Request__ListAccount uid;
+     Request__TakeOrder   uid oid;
+     Request__MakeOrder   uid bt ba st ax;
+     Request__Deposit     uid bt ba;
+     Request__Withdraw    uid st ax].
